tracking undelegations as well, based on Kushal's design. working on the proof where that change seems to be needed. the proof also seems to need the assumption that the txs in the extension span K or fewer blocks

monadproofs/proofs/reservebal.v
@@ -55,12 +55,13 @@ Definition value (t: TxWithHdr): N := w256_to_N (block.tr_value (fst (snd t))).
 
 Definition K : N. Proof. Admitted.
 
-Definition addrsDelegatedByTx  (tx: TxWithHdr) : list evm.address. Proof. Admitted.
+Definition addrsDelUndelByTx  (tx: TxWithHdr) : list evm.address. Proof. Admitted.
 
-Definition txDelegatesAddr (addr: evm.address) (tx: TxWithHdr) : bool :=
-  bool_decide (addr ∈ addrsDelegatedByTx tx).
+Definition txDelUndelAddr (addr: evm.address) (tx: TxWithHdr) : bool :=
+  bool_decide (addr ∈ addrsDelUndelByTx tx).
 
-Opaque txDelegatesAddr.
+
+Opaque txDelUndelAddr.
 
 
 (*
@@ -103,8 +104,8 @@ Definition indexWithinK (proj: AccountM -> option Indices) (state : StateOfAccou
 Definition existsTxWithinK (state : StateOfAccounts)  (tx: TxWithHdr) : bool :=
   indexWithinK lastTxInBlockIndex state tx.
 
-Definition existsDelegatingTxWithinK (state : StateOfAccounts)  (tx: TxWithHdr) : bool :=
-  indexWithinK  lastDelegatedInBlockIndex state tx.
+Definition existsDelUndelTxWithinK (state : StateOfAccounts)  (tx: TxWithHdr) : bool :=
+  indexWithinK  lastDelUndelInBlockIndex state tx.
 
 (*
 [StateOfAccounts] already stores the [Indices] (block index, tx index) of the the last tx from an account.
@@ -122,8 +123,8 @@ t n-k+1
 Definition isAllowedToEmpty
   (state : StateOfAccounts) (intermediateTxsSinceState: list TxWithHdr)  (tx: TxWithHdr) : bool :=
   let delegated := (addrDelegated state (sender tx))
-                   || existsDelegatingTxWithinK state tx
-                   || bool_decide  ((sender tx) ∈ flat_map addrsDelegatedByTx (tx::intermediateTxsSinceState))
+                   || existsDelUndelTxWithinK state tx
+                   || bool_decide  ((sender tx) ∈ flat_map addrsDelUndelByTx (tx::intermediateTxsSinceState))
   in
   let existsSameSenderTxInWindow :=
     (existsTxWithinK state tx)
@@ -154,6 +155,18 @@ Proof using.
   case_bool_decide; auto.
 Qed.
 
+(*
+Lemma updateKeyLkp4  {T} `{c: Countable T} {V} {inhv: Inhabited V} (m: gmap T V) (a b: T) (f: V -> V) :
+  (updateKey m a f) !! b = if (bool_decide (a=b)) then option_map f  (m !! a) else m !! b.
+Proof using.
+  unfold updateKey.
+  autorewrite with syntactic;[| exact inhabitant].
+  case_bool_decide; auto.
+  reflexivity.
+Qed.
+ *)
+
+(*
 Lemma updateKeyLkp  {T} `{c: Countable T} {V} {inhv: Inhabited V} (m: gmap T V) (a: T) (f: V -> V) :
   updateKey m a f !! a = Some (f (m !!! a)).
 Proof using.
@@ -162,6 +175,7 @@ Proof using.
   reflexivity.
 Qed.
 
+ *)
 
 (*
 Fixpoint maxTotalReserveDippableDebitLold (knownBlocks: gmap N Block) (latestKnownState : StateOfAccounts) (postStateAccountedSuffix rest: list TxWithHdr) (a: evm.address) : N:=
@@ -256,8 +270,8 @@ Definition DippedTooMuchIntoReserve (t: TxWithHdr): TransactionResult. Proof. Ad
 
 Definition addrConsideredDelegated  (state: evm.GlobalState) (tx : TxWithHdr) : bool :=
   (addrDelegated state (sender tx))
-                   || (bool_decide (sender tx ∈ addrsDelegatedByTx tx))
-                   || existsDelegatingTxWithinK state tx.
+                   || (bool_decide (sender tx ∈ addrsDelUndelByTx tx))
+                   || existsDelUndelTxWithinK state tx.
 Definition isAllowedToEmptyExec
   (state : StateOfAccounts)  (tx: TxWithHdr) : bool :=
   (negb (addrConsideredDelegated state tx)) && (negb (existsTxWithinK state tx)).
@@ -382,7 +396,7 @@ Proof. Admitted.
 (* what happens if the tx undelegates something. maybe weaken it *)
 Lemma execTxDelegationUpd tx s:
   let '(sf, r) :=  execValidatedTx s tx in
-  (forall ac, addrDelegated sf ac <-> addrDelegated s ac || bool_decide (ac ∈ (addrsDelegatedByTx tx))).
+  (forall ac, addrDelegated sf ac <-> addrDelegated s ac || bool_decide (ac ∈ (addrsDelUndelByTx tx))).
 Proof. Admitted.
 
 Lemma execTxCannotDebitNonDelegatedNonContractAccounts tx s:
@@ -406,7 +420,73 @@ Proof using.
   intros. subst. reflexivity.
 Qed.
 
-Lemma debitLeq extension s sf tx rest:
+(* technically, the lemma is unprobable, however, we can prove a Proper lemma about the context *)
+Lemma gmapEquiv {T} `{c: Countable T} {V} {inhv: Inhabited V} (m1 m2: gmap T V) :
+  (forall a, m1 !!! a = m2 !!! a) -> m1 =m2.
+Proof. Admitted.
+
+Hint Rewrite @elem_of_cons: syntactic.
+
+Set Nested Proofs Allowed.
+
+    Lemma lastTxInBlockIndexUpd s txlast:
+      option_bind _ _ lastTxInBlockIndex ((execValidatedTx s txlast).1 !! sender txlast)
+      = Some (indicesOfTx txlast).
+    Proof using. Admitted.
+
+Lemma isAllowedToEmpty2 s txlast rest txnext:
+  let sf :=  fst (execValidatedTx s txlast) in 
+  isAllowedToEmpty sf rest txnext = isAllowedToEmpty s (txlast :: rest) txnext.
+Proof using.
+  unfold isAllowedToEmpty.
+  simpl.
+  autorewrite with syntactic.
+  destruct (decide (sender txnext = sender txlast)).
+  {
+    assert ((bool_decide (sender txnext ∈ sender txlast :: map sender rest)) = true) as Hf.
+    {
+      rewrite bool_decide_true; auto.
+      set_solver.
+    }
+
+    rewrite Hf.
+    autorewrite with syntactic.
+    match goal with
+    |  |-  _ && ?r = false =>
+         assert (r=false) as Hrf
+    end;
+    [|  rewrite Hrf; autorewrite with syntactic; reflexivity].
+    unfold existsTxWithinK.
+    unfold indexWithinK.
+    rwHypsP.
+    rewrite lastTxInBlockIndexUpd.
+    simpl.
+    unfold indLe. simpl.
+    simpl.
+    rewrite bool_decide_true;[reflexivity|].
+    split_and !; try lia.
+
+(*
+  number txnext.1 - K ≤ number txlast.1
+
+goal 2 (ID 904) is:
+ number txlast.1 ≤ number txnext.1
+goal 3 (ID 905) is:
+ txlast.2.2 ≤ txnext.2.2
+*)    
+    lia.
+
+    rewrite bool_decide_decide.
+    resolveDecide congruence.
+    symmetry.
+    rwHyps.
+  Search bool_decide iff.
+  
+  simpl. f_equiv.
+Abort.
+
+Lemma debitLeq extension s tx rest:
+  let sf :=  fst (execValidatedTx s tx) in 
   (maxTotalReserveDippableDebitL  sf rest extension)
   = (maxTotalReserveDippableDebitL  s (tx::rest) extension).
 Proof using.
@@ -415,19 +495,29 @@ Proof using.
   intros.
   simpl.
   rewrite IHextension.
-  (*
-  f_equiv.
+  apply gmapEquiv.
+  intros ad.
+  repeat rewrite updateKeyLkp3.
+  case_bool_decide; auto;[].
   unfold updateTotals.
   simpl.
-  f_equiv.
-  unfold maxTotalReserveDippableDebit.
   apply ite_fequiv; try reflexivity.
   unfold isAllowedToEmpty.
   simpl. f_equiv.
+  2:{
+    simpl.
+    
+    Lemma existsTxWithinKUpd s tx a:
+      let sf :=  fst (execValidatedTx s tx) in 
+      existsTxWithinK sf a = existsTxWithinK s a.
   - admit. (* existsDelegatingTxWithinK sf a <-> (existsDelegatingTxWithinK s a) ||  addrsDelegatedByTx tx *)
   - admit. (* similar prop for [existsTxWithinK] *) *)
 Admitted. (* seems easy *)
 
+  Search (gmap _ _) (_ = _).
+  Search  gmap Proper.
+  Search updateKey.
+  f_equiv.
 #[global] Instance inhadd: Inhabited evm.address := populate word160.word160_default.
 Lemma moveForallIn {T} {inh:Inhabited T} P (Q: T -> Prop):
   (forall x, P /\ Q x)  -> P /\ forall x, Q x.
